To find the root of the quadratic equation $\(n^2 + n - 2T = 0\)$, where \(2T\) is a constant, we can use the quadratic formula:

$\[ n = \frac{{-b \pm \sqrt{{b^2 - 4ac}}}}{{2a}} \]$
In this equation, \(a = 1\), \(b = 1\), and \(c = -2T\).

Substitute these values into the quadratic formula:

$\[ n = \frac{{-(1) \pm \sqrt{{(1)^2 - 4(1)(-2T)}}}}{{2(1)}} \]$

$\[ n = \frac{{-1 \pm \sqrt{{1 + 8T}}}}{2} \]$

So, the roots of the equation are:

$\[ n = \frac{{-1 + \sqrt{{1 + 8T}}}}{2} \]$

$\[ n = \frac{{-1 - \sqrt{{1 + 8T}}}}{2} \]$

These are the roots of the quadratic equation $\(n^2 + n - 2T = 0\)$.
